examples/pseudo_bool/cp_encoding/cp_to_ilp_primScript.sml
@@ -7,10 +7,33 @@ Libs
 Ancestors
   pbc cp ilp cp_to_ilp
 
+Definition lt_var_def[simp]:
+  lt_var name =
+    INR (name, Flag (strlit "lt"))
+End
+
+Definition gt_var_def[simp]:
+  gt_var name =
+    INR (name, Flag (strlit "gt"))
+End
+
 Definition ne_var_def[simp]:
   ne_var name =
     INR (name, Flag (strlit "ne"))
 End
+
+Definition at_least_one_def:
+  at_least_one ls =
+    ([], MAP (λl. (1,l)) ls, 1)
+End
+
+Theorem at_least_one_sem[simp]:
+  iconstraint_sem (at_least_one ls) (wi,wb) ⇔
+  ∃l. MEM l ls ∧ lit wb l
+Proof
+  rw[iconstraint_sem_def,at_least_one_def,eval_lin_term_def]>>
+  simp[MAP_MAP_o,o_DEF]
+QED
 
 Definition encode_equal_def:
   encode_equal bnd Zr X Y name =
@@ -28,12 +51,13 @@ Definition encode_equal_def:
     encode_ge bnd Z 1 ++
     MAP (bits_imply bnd [Pos (INL (Ge Z 1))]) constr ++
     [
-      bits_imply bnd
-        [Neg (INL (Ge Z 1)); Pos (ne_var name)]
-          (mk_constraint_ge 1 X (-1) Y 1);
-      bits_imply bnd
-        [Neg (INL (Ge Z 1)); Neg (ne_var name)]
-          (mk_constraint_ge 1 Y (-1) X 1)
+      bits_imply bnd [Pos (gt_var name)]
+        (mk_constraint_ge 1 X (-1) Y 1);
+      bits_imply bnd [Pos (lt_var name)]
+         (mk_constraint_ge 1 Y (-1) X 1);
+      at_least_one
+        [Pos (lt_var name); Pos (gt_var name);
+          Pos (INL (Ge Z 1))];
     ]
 End
 
@@ -46,10 +70,13 @@ Theorem encode_equal_sem_1:
     (encode_equal bnd Zr X Y name)
 Proof
   rw[reify_sem_def,encode_equal_def]>>
-  gvs[AllCasePreds(),reify_avar_def,reify_reif_def,reify_flag_def]
+  gvs[AllCasePreds(),reify_avar_def,reify_reif_def,reify_flag_def,iconstraint_sem_def]
   >- intLib.ARITH_TAC
   >- intLib.ARITH_TAC
-  >- intLib.ARITH_TAC
+  >- (
+    rw[oneline b2i_def]>>
+    simp[SF DNF_ss,reify_avar_def,reify_flag_def,reify_reif_def]>>
+    intLib.ARITH_TAC)
 QED
 
 Theorem encode_equal_sem_2:
@@ -60,13 +87,8 @@ Theorem encode_equal_sem_2:
     (varc wi X = varc wi Y)
 Proof
   rw[reify_sem_def,encode_equal_def]>>
-  every_case_tac>>gvs[]
-  >-  intLib.ARITH_TAC
-  >-  intLib.ARITH_TAC>>
-  rename1`wb (INR f)`>>
-  Cases_on`wb (INR f)`>>gvs[]
-  >-  intLib.ARITH_TAC
-  >-  intLib.ARITH_TAC
+  every_case_tac>>gvs[]>>
+  intLib.ARITH_TAC
 QED
 
 Definition encode_not_equal_def:
@@ -81,14 +103,11 @@ Definition encode_not_equal_def:
     ]
   | SOME (INL Z) =>
     encode_ge bnd Z 1 ++
-    [
-      bits_imply bnd
-        [Pos (INL (Ge Z 1)); Pos (ne_var name)]
-          xgty;
-      bits_imply bnd
-        [Pos (INL (Ge Z 1)); Neg (ne_var name)]
-          ygtx
-    ]
+    bimply_bits bnd [Pos (gt_var name)] xgty ++
+    bimply_bits bnd [Pos (lt_var name)] ygtx ++
+    [at_least_one
+      [Pos (lt_var name); Pos (gt_var name);
+        Neg (INL (Ge Z 1))]]
   | SOME (INR Z) =>
     encode_ge bnd Z 1 ++
     MAP (bits_imply bnd [Neg (INL (Ge Z 1))])
@@ -97,12 +116,11 @@ Definition encode_not_equal_def:
         mk_constraint_ge 1 (Y) (-1) (X) 0
       ] ++
     [
-      bits_imply bnd
-        [Pos (INL (Ge Z 1)); Pos (ne_var name)]
-          xgty;
-      bits_imply bnd
-        [Pos (INL (Ge Z 1)); Neg (ne_var name)]
-          ygtx
+      bits_imply bnd [Pos (gt_var name)] xgty;
+      bits_imply bnd [Pos (lt_var name)] ygtx;
+      at_least_one
+        [Pos (lt_var name); Pos (gt_var name);
+          Neg (INL (Ge Z 1))];
     ]
 End
 
@@ -116,9 +134,13 @@ Theorem encode_not_equal_sem_1:
 Proof
   rw[reify_sem_def,encode_not_equal_def]>>
   gvs[AllCasePreds(),reify_avar_def,reify_flag_def,reify_reif_def]
-  >-  intLib.ARITH_TAC
-  >-  intLib.ARITH_TAC
-  >-  intLib.ARITH_TAC
+  >- intLib.ARITH_TAC
+  >- (
+    simp[SF DNF_ss,reify_avar_def,reify_flag_def,reify_reif_def]>>
+    intLib.ARITH_TAC)
+  >- (
+    simp[SF DNF_ss,reify_avar_def,reify_flag_def,reify_reif_def]>>
+    intLib.ARITH_TAC)
 QED
 
 Theorem encode_not_equal_sem_2:
@@ -130,17 +152,12 @@ Theorem encode_not_equal_sem_2:
 Proof
   rw[reify_sem_def,encode_not_equal_def]>>
   gvs[AllCasePreds(),reify_avar_def,reify_flag_def,reify_reif_def]>>
-  rename1`INR f`>>
   every_case_tac>>gvs[]
   >- (
+    rename1`INR f`>>
     Cases_on`wb (INR f)`>>gvs[]>>
-    intLib.ARITH_TAC)
-  >- (
-    Cases_on`wb (INR f)`>>gvs[]>>
-    intLib.ARITH_TAC)
-  >- (
-    Cases_on`wb (INR f)`>>gvs[]>>
-    intLib.ARITH_TAC)
+    intLib.ARITH_TAC)>>
+  intLib.ARITH_TAC
 QED
 
 Definition encode_prim_constr_def:
